

## Task 1

$$y = \exp[\exp(x) + \exp(x)^2] + \sin[\exp(x) + \exp(x)^2]$$

a)  $f_1 = \exp(x)$

$$f_2 = f_1^2$$

$$f_3 = f_1 + f_2$$

$$f_4 = \exp(f_3)$$

$$f_5 = \sin(f_3)$$

$$y = f_4 + f_5$$

b)  $\frac{\partial f_1}{\partial x} = \exp(x)$

$$\frac{\partial f_2}{\partial x} = \frac{\partial f_1}{\partial x} \frac{\partial f_1}{\partial x} = 2\exp(x)\exp(x) = 2\exp(2x)$$

$$\frac{\partial f_3}{\partial x} = \frac{\partial f_1}{\partial x} + \frac{\partial f_2}{\partial x} = \exp(x) + 2\exp(x)$$

$$\frac{\partial f_4}{\partial x} = \frac{\partial f_4}{\partial f_3} \frac{\partial f_3}{\partial x} = \exp(f_3) [\exp(x) + 2\exp(x)]$$

$$\frac{\partial f_5}{\partial x} = \frac{\partial f_5}{\partial f_3} \frac{\partial f_3}{\partial x} = \cos(f_3) [\exp(x) + 2\exp(x)]$$

$$\frac{\partial y}{\partial x} = \frac{\partial f_4}{\partial x} + \frac{\partial f_5}{\partial x} = \exp(f_3) [\exp(x) + 2\exp(x)] + \cos(f_3) [\exp(x) + 2\exp(x)]$$

$$= \exp[\exp(x) + \exp(x)^2] [\exp(x) + 2\exp(x)] + \cos[\exp(x) + \exp(x)^2] [\exp(x) + 2\exp(x)]$$

c)  $\frac{\partial y}{\partial f_5} = f_4$

$$\frac{\partial y}{\partial f_4} = f_5$$

$$\frac{\partial y}{\partial f_3} = \frac{\partial f_4}{\partial f_3} + \frac{\partial f_5}{\partial f_3} = \exp(f_3) + \cos(f_3)$$

$$\frac{\partial y}{\partial f_2} = \frac{\partial f_4}{\partial f_2} + \frac{\partial f_5}{\partial f_2} = \frac{\partial f_4}{\partial f_3} \frac{\partial f_3}{\partial f_2} + \frac{\partial f_5}{\partial f_3} \frac{\partial f_3}{\partial f_2} = \exp(f_3) f_1 + \cos(f_3) f_1$$

$$\frac{\partial y}{\partial f_1} = \frac{\partial f_4}{\partial f_1} + \frac{\partial f_5}{\partial f_1} = \frac{\partial f_4}{\partial f_3} \frac{\partial f_3}{\partial f_1} + \frac{\partial f_5}{\partial f_3} \frac{\partial f_3}{\partial f_1} = \exp(f_3) f_2 + \cos(f_3) f_2$$

$$\begin{aligned} \frac{\partial y}{\partial x} &= \frac{\partial f_4}{\partial x} + \frac{\partial f_5}{\partial x} = \frac{\partial f_4}{\partial f_3} \frac{\partial f_3}{\partial x} + \frac{\partial f_5}{\partial f_3} \frac{\partial f_3}{\partial x} = \frac{\partial f_4}{\partial f_3} \left( \frac{\partial f_1}{\partial x} + \frac{\partial f_2}{\partial x} \right) + \frac{\partial f_5}{\partial f_3} \left( \frac{\partial f_1}{\partial x} + \frac{\partial f_2}{\partial x} \right) \\ &= \exp[\exp(x) + \exp(x)^2] [\exp(x) + 2\exp(x)] + \cos[\exp(x) + \exp(x)^2] [\exp(x) + 2\exp(x)] \end{aligned}$$

## Task 2

a)  $\phi_{t+1} \leftarrow \phi_t - \alpha \frac{\tilde{m}_{t+1}}{\sqrt{\tilde{v}_{t+1}} + \epsilon}$  normalization of the modified grad

$$\tilde{m}_{t+1} \leftarrow \frac{m_{t+1}}{1 - \beta^{t+1}}$$

$$\tilde{v}_{t+1} \leftarrow \frac{v_{t+1}}{1 - \beta^{t+1}}$$

, mod. grad to avoid 0 at beginning

$$m_{t+1} \leftarrow \beta m_t + (1-\beta) \frac{\partial L(\phi_t)}{\partial \phi}, \text{ med. grad to avoid 0 at beginning}$$

$$\tilde{v}_{t+1} \leftarrow \frac{v_{t+1}}{1-\gamma^{t+1}}$$

$$m_{t+1} \leftarrow \beta m_t + (1-\beta) \frac{\partial L(\phi_t)}{\partial \phi}$$

$$v_{t+1} \leftarrow \gamma v_t + (1-\gamma) \left( \frac{\partial L(\phi_t)}{\partial \phi} \right)^2 \text{ add momentum}$$

$$\begin{aligned} b) \phi_1 &\leftarrow \phi_0 - \alpha \frac{\tilde{m}_1}{\|\tilde{v}_1\| + \epsilon}, \tilde{m}_1 \leftarrow \frac{m_1}{1-\beta}, \tilde{v}_1 \leftarrow \frac{v_1}{1-\gamma} \\ &\leftarrow \phi_0 - \alpha \frac{m_1}{\|v_1\| + \epsilon} \frac{1-\gamma}{1-\beta}, m_1 = (1-\beta) \frac{\partial L}{\partial \phi}, v_1 = (1-\gamma) \left( \frac{\partial L}{\partial \phi} \right)^2 \\ &\leftarrow \phi_0 - \alpha \frac{\partial L / \partial \phi}{\|\partial L / \partial \phi\| + \epsilon} \approx \phi_0 - \alpha \operatorname{sgn}(\partial L / \partial \phi) \approx \phi_0 - \operatorname{sgn}(g) \\ &\Rightarrow \text{update dep only on } \operatorname{sgn}(g) \end{aligned}$$

c) keep  $\epsilon$

d) i) put in loss:  $g_t = \frac{\partial L}{\partial w} + \lambda w$

ii) direct weight decay:  $w \leftarrow \alpha \lambda w$  (AdamW)

AdamW is better.  $\Leftarrow$  matches desired effect of  $L_2$  reg

### Task 3

$$b) p(y|x, \theta) = \mathcal{N}(y | f_\mu(x), \sigma^2)$$

$$\begin{aligned} -\log[p(y|x, \theta)] &= \frac{1}{2\sigma^2} [y - f_y(x)]^2 + \frac{1}{2} \log(\sigma^2) + \text{const}, \sigma = \text{const} \\ &= \frac{1}{C} \underbrace{[y - f_y(x)]^2}_{\text{MSE}} + \text{const} \end{aligned}$$

$$e) f_\mu(x_i) = \mu(x_i), f_{\sigma^2}(x_i) = \sigma^2(x_i)$$

$$p(y|x, \theta) = \mathcal{N}(y | f_\mu(x), f_{\sigma^2}(x))$$

$$\Rightarrow -\log p(y|x, \theta) = \frac{1}{2} \log(2\pi) + \frac{1}{2} \log \sigma^2 + \frac{(y_i - \mu_i)^2}{2\sigma_i^2}$$

$$\Rightarrow -\log p(y_i | x_i, \theta) = \frac{1}{2} \log(2\pi) + \frac{1}{2} \log \sigma_i^2 + \frac{(y_i - \mu_i)^2}{2\sigma_i^2}$$

$\Rightarrow$  total for data set:

$$\begin{aligned} L &= -\frac{1}{2} \sum_{i=1}^n \left[ \log(2\pi) + \log \sigma_i^2 + \frac{(y_i - \mu_i)^2}{\sigma_i^2} \right] \\ &= -\frac{1}{2} \sum_{i=1}^n \left[ \log \sigma_i^2 + \frac{(y_i - \mu_i)^2}{\sigma_i^2} \right] + \text{const} \end{aligned}$$

Remark to nb: My export to .pdf is broken and I could not fix it in time. Therefore the nb will only be a jupyter nb.